Updates and improvements to the l3-machine-code decompilation tools.

examples/l3-machine-code/arm/decompiler/arm_decompLib.sig
@@ -1,6 +1,7 @@
 signature arm_decompLib =
 sig
 
+    val config_for_fast   : unit -> unit
     val l3_arm_triples    : string -> Thm.thm list
     val l3_arm_tools      : helperLib.decompiler_tools
     val l3_arm_decompile  : string -> Term.term quotation -> Thm.thm * Thm.thm
