examples/l3-machine-code/arm/decompiler/arm_relLib.sig
@@ -1,0 +1,8 @@
+signature arm_relLib =
+sig
+
+    val l3_triple: string -> (Thm.thm * int * int option) *
+                             (Thm.thm * int * int option) option
+    val swap_primes: Term.term -> Term.term
+
+end
