examples/l3-machine-code/arm/decompiler/arm_relLib.sml
@@ -1,16 +1,13 @@
-structure arm_relLib =
+structure arm_relLib :> arm_relLib =
 struct
 
 open HolKernel Parse boolLib bossLib Lib
-open armTheory armLib arm_stepTheory pred_setTheory pairTheory optionTheory
-open arithmeticTheory wordsTheory wordsLib addressTheory combinTheory pairSyntax
-open sumTheory whileTheory
 
 open arm_relTheory progTheory helperLib arm_decompLib
 
-local
-
 val ERR = Feedback.mk_HOL_ERR "arm_relLib"
+
+(* ------------------------------------------------------------------------ *)
 
 val cond_var = mk_var ("cond", ``:bool``)
 val r15 = mk_var ("r15", ``:word32``)
@@ -20,12 +17,10 @@ val (spec,_,_,_) = arm_decompLib.l3_arm_tools
 val arm_assert =
    ARM_ASSERT_def
    |> SPEC_ALL
-   |> REWRITE_RULE [arm_FP_REGS_def]
    |> Conv.CONV_RULE (Conv.RHS_CONV helperLib.STAR_AC_CONV)
    |> GSYM
 
 val targets = progSyntax.strip_star (utilsLib.lhsc arm_assert)
-val fv_spec_tm = free_vars (Thm.concl arm_assert)
 
 val precond_thm = Q.prove(
    `!b. precond b = cond (Abbrev b): 'a set set`,
@@ -38,7 +33,8 @@ val PAIR_LEMMA = Q.prove(
    SIMP_TAC std_ss [])
 
 fun find_match [] tm = fail()
-  | find_match (x::xs) tm = match_term x tm handle HOL_ERR _ => find_match xs tm
+  | find_match (x::xs) tm =
+       fst (match_term x tm) handle HOL_ERR _ => find_match xs tm
 
 fun first_r_eq x = rand o Lib.first (equal (rator x) o rator)
 
@@ -60,30 +56,39 @@ val INTRO_TRIPLE_RULE =
    FORCE_DISCH_ALL
 
 (* abbreviate posts *)
-fun abbrev_conv ignore pat post =
-  if ignore pat
+fun abbrev_conv pat post =
+  if pat = r15
      then ALL_CONV post
   else if is_var pat
      then if pat = post
              then ALL_CONV post
           else ASSUME (mk_eq (post, add_prime pat))
   else if is_comb pat
-     then (RAND_CONV (abbrev_conv ignore (rand pat))
-           THENC RATOR_CONV (abbrev_conv ignore (rator pat))) post
+     then (RAND_CONV (abbrev_conv (rand pat))
+           THENC RATOR_CONV (abbrev_conv (rator pat))) post
   else if pat = post
      then ALL_CONV post
   else NO_CONV post
 
-fun old_to_new th =
+val precond_rule =
+   UNDISCH_ALL o
+   Conv.CONV_RULE
+      (helperLib.PRE_CONV
+          (PURE_ONCE_REWRITE_CONV [precond_thm]
+           THENC helperLib.MERGE_CONDS_CONV)
+       THENC PURE_ONCE_REWRITE_CONV [SPEC_MOVE_COND])
+
+fun spec_to_triple_rule th =
    let
-      val th =
-         th |> SIMP_RULE (std_ss++sep_cond_ss) [precond_thm]
-            |> REWRITE_RULE [SPEC_MOVE_COND]
-            |> UNDISCH_ALL
+      val th = precond_rule th
       val fnd =
          find_match (progSyntax.strip_star (progSyntax.dest_pre (Thm.concl th)))
-      val frame = progSyntax.list_mk_star (List.filter (not o can fnd) targets)
-      val xs = List.concat (List.mapPartial (Lib.total (fst o fnd)) targets)
+      val (xs, frm) =
+         List.foldr (fn (t, (sbst, frm)) =>
+            case Lib.total fnd t of
+               SOME s => (sbst @ s, frm)
+             | NONE => (sbst, t :: frm)) ([], []) targets
+      val frame = progSyntax.list_mk_star frm
       val th =
          th |> INST xs
             |> SPECC_FRAME_RULE frame
@@ -115,29 +120,34 @@ fun old_to_new th =
             |> INTRO_TRIPLE_RULE
       val pat = th |> concl |> rator |> rator |> rand
    in
-      th |> CONV_RULE (RAND_CONV (abbrev_conv (Lib.equal r15) pat))
+      th |> CONV_RULE (RAND_CONV (abbrev_conv pat))
          |> DISCH_ALL
          |> repeat (MATCH_MP PAIR_LEMMA)
          |> UNDISCH_ALL
    end
 
-in
-
 val l3_triple =
    (* cache *)
      (fn hex =>
          (case spec hex of
-             ((th1,x1,y1 as SOME _), NONE) => ((old_to_new th1,x1,y1), NONE)
+             ((th1,x1,y1 as SOME _), NONE) =>
+                 ((spec_to_triple_rule th1,x1,y1), NONE)
            | ((th1,x1,y1 as SOME _), SOME (th2,x2,y2)) =>
-                 ((old_to_new th1,x1,y1), SOME (old_to_new th2,x2,y2))
+                 ((spec_to_triple_rule th1,x1,y1),
+                  SOME (spec_to_triple_rule th2,x2,y2))
            | _ => fail())
          handle HOL_ERR _ => raise ERR "l3_triple" hex)
 
-val (swap_primes,SWAP_PRIMES_RULE) = let
-  val vs = (cond_var :: fv_spec_tm) |> map (fn v => (v,add_prime v))
-  val ss = map (fn (x,y) => x |-> y) vs @ map (fn (x,y) => y |-> x) vs
-  in (subst ss, INST ss) end
+val fv_spec_tm = free_vars (Thm.concl arm_assert)
 
-end
+val (swap_primes,SWAP_PRIMES_RULE) =
+   let
+      val vs = (cond_var :: fv_spec_tm) |> map (fn v => (v,add_prime v))
+      val ss = map (fn (x,y) => x |-> y) vs @ map (fn (x,y) => y |-> x) vs
+   in
+      (subst ss, INST ss)
+   end
+
+(* ------------------------------------------------------------------------ *)
 
 end
