examples/l3-machine-code/arm/step/arm_configLib.sig
@@ -1,6 +1,7 @@
 signature arm_configLib =
 sig
    include Abbrev
+   val map_options: string -> bool * bool * bool
    val mk_arm_const: string -> term
    val mk_arm_type: string -> hol_type
    val mk_config_terms: string -> term list
