examples/l3-machine-code/x64/prog/x64_progScript.sml
@@ -1,16 +1,19 @@
 open HolKernel boolLib bossLib
-open stateLib x64_stepTheory
+open lcsymtacs set_sepTheory progTheory pred_setTheory stateLib x64_stepTheory
 
 val () = new_theory "x64_prog"
+
+infix \\
+val op \\ = op THEN;
 
 (* ------------------------------------------------------------------------ *)
 
 val _ = stateLib.sep_definitions "x64" [] [] x64_stepTheory.NextStateX64_def
 
 val x64_mem_def = Define`
-   x64_mem a (i: word8 list) =
-   set (GENLIST (\x. (x64_c_MEM (a + n2w x),
-                      x64_d_word8_option (SOME (EL x i)))) (LENGTH i))`
+   x64_mem a (l: word8 list) =
+   set (GENLIST (\i. (x64_c_MEM (a + n2w i),
+                      x64_d_word8_option (SOME (EL i l)))) (LENGTH l))`
 
 val x64_instr_def = Define`
    x64_instr (a, i) =
@@ -25,10 +28,11 @@ val x64_mem32_def = Define`
    x64_mem32 a (v: word32) =
    { x64_mem a [(7 >< 0) v; (15 >< 8) v; (23 >< 16) v; (31 >< 24) v] }`
 
+val v8 = ``[( 7 ><  0) v; (15 ><  8) v; (23 >< 16) v; (31 >< 24) (v:word64);
+            (39 >< 32) v; (47 >< 40) v; (55 >< 48) v; (63 >< 56) v]:word8 list``
+
 val x64_mem64_def = Define`
-   x64_mem64 a (v: word64) =
-   { x64_mem a [( 7 ><  0) v; (15 ><  8) v; (23 >< 16) v; (31 >< 24) v;
-                (39 >< 32) v; (47 >< 40) v; (55 >< 48) v; (63 >< 56) v] }`
+   x64_mem64 a (v: word64) = { x64_mem a ^v8 }`
 
 val X64_MODEL_def = Define`
   X64_MODEL = (STATE x64_proj, NEXT_REL (=) NextStateX64, x64_instr,
@@ -39,6 +43,116 @@ val X64_IMP_SPEC = Theory.save_thm ("X64_IMP_SPEC",
    |> Q.ISPECL [`x64_proj`, `NextStateX64`, `x64_instr`]
    |> REWRITE_RULE [GSYM X64_MODEL_def]
    )
+
+(* ------------------------------------------------------------------------ *)
+
+val x64_MEM_def = DB.definition "x64_MEM_def"
+
+val (x64_BYTE_MEMORY_def, x64_BYTE_MEMORY_INSERT) =
+   stateLib.define_map_component ("x64_BYTE_MEMORY", "bmem", x64_MEM_def)
+
+val x64_MEMORY_def = Define`
+  x64_MEMORY dmem mem =
+  { BIGUNION { BIGUNION (x64_mem64 a (mem a)) | a IN dmem /\ (a && 7w = 0w)} }`
+
+val x64_PC_def = Define`
+   x64_PC pc = x64_RIP pc * x64_exception NoException`
+
+val x64_ALL_EFLAGS_def = Define `
+  x64_ALL_EFLAGS =
+    ~(x64_EFLAGS Z_AF) *
+    ~(x64_EFLAGS Z_CF) *
+    ~(x64_EFLAGS Z_OF) *
+    ~(x64_EFLAGS Z_PF) *
+    ~(x64_EFLAGS Z_SF) *
+    ~(x64_EFLAGS Z_ZF)`
+
+(* ------------------------------------------------------------------------ *)
+
+val thm =
+   MATCH_MP
+     (stateTheory.MAPPED_COMPONENT_INSERT
+      |> Q.ISPECL
+            [`\a:word64. a && 7w = 0w`, `8`, `\a i. x64_c_MEM (a + n2w i)`,
+             `\v:word64 i.  x64_d_word8_option (SOME (EL i ^v8))`, `x64_mem64`,
+             `x64_MEMORY`]
+      |> Conv.CONV_RULE (Conv.LAND_CONV (SIMP_CONV std_ss [])))
+     (REWRITE_RULE [x64_mem_def, EVAL ``LENGTH [a; b; c; d; e; f; g; h]``]
+         x64_mem64_def)
+
+val lem1 = Q.prove(
+   `!i. i < 8 ==> n2w i <+ (8w: word64)`,
+   simp [wordsTheory.word_lo_n2w])
+
+val lem2 =
+   blastLib.BBLAST_PROVE
+      ``(7w && a = 0w:word64) /\ (7w && b = 0w) /\ x <+ 8w /\ y <+ 8w ==>
+        ((a + x = b + y) = (a = b) /\ (x = y))``
+
+(* Need ``(\a. ..) c`` below for automation to work *)
+val x64_MEMORY_INSERT = Q.store_thm("x64_MEMORY_INSERT",
+   `!f df c d.
+     c IN df /\ (\a. a && 7w = 0w) c ==>
+     (x64_mem64 c d * x64_MEMORY (df DELETE c) f = x64_MEMORY df ((c =+ d) f))`,
+   match_mp_tac thm
+   \\ rw [x64_MEMORY_def]
+   \\ `(i = j) = (n2w i = n2w j: word64)` by simp []
+   \\ asm_rewrite_tac []
+   \\ match_mp_tac lem2
+   \\ simp [lem1]
+   )
+
+(* ------------------------------------------------------------------------ *)
+
+val x64_mem64_APPEND = Q.prove(
+   `x64_mem32 a v * x64_mem32 (a + 4w) ((63 >< 32) w) =
+    x64_mem64 a ((((63 >< 32) w):word32) @@ v)`,
+   SIMP_TAC std_ss [x64_mem64_def, x64_mem32_def]
+   \\ SIMP_TAC std_ss [GSYM stateTheory.SEP_EQ_SINGLETON]
+   \\ MATCH_MP_TAC stateTheory.SEP_EQ_STAR
+   \\ SIMP_TAC std_ss [stateTheory.SEP_EQ_SINGLETON, BIGUNION_SING,
+                       DISJOINT_DEF, EXTENSION]
+   \\ SIMP_TAC (srw_ss())
+         [PULL_EXISTS, combinTheory.APPLY_UPDATE_THM, x64_mem_def]
+   \\ REPEAT STRIP_TAC
+   \\ FULL_SIMP_TAC std_ss []
+   THEN1 (REPEAT STRIP_TAC
+          \\ EQ_TAC
+          \\ REPEAT STRIP_TAC
+          \\ FULL_SIMP_TAC (srw_ss()) [addressTheory.WORD_EQ_ADD_CANCEL]
+          \\ blastLib.BBLAST_TAC)
+   \\ CCONTR_TAC
+   \\ FULL_SIMP_TAC std_ss []
+   \\ FULL_SIMP_TAC (srw_ss()) [addressTheory.WORD_EQ_ADD_CANCEL]);
+
+val lemma = blastLib.BBLAST_PROVE
+   ``(((63 >< 32) w):word32) @@ ((w2w w):word32) = (w:word64)``
+
+val lemma2 = blastLib.BBLAST_PROVE
+   ``((((63 :num) >< (32 :num))
+        (((((63 :num) >< (32 :num)) (w:word64) :word32)
+           @@ (v:word32)) :word64) :word32) =
+     ((63 >< 32) w):word32) /\
+     (w2w (((((63 >< 32) w):word32) @@ v):word64) = v)``
+
+val x64_mem32_READ_EXTEND = Q.store_thm("x64_mem32_READ_EXTEND",
+   `SPEC m (p * x64_mem32 a (w2w w)) c (q * x64_mem32 a (w2w w)) ==>
+    SPEC m (p * x64_mem64 a w) c (q * x64_mem64 a w)`,
+   REPEAT STRIP_TAC
+   \\ ONCE_REWRITE_TAC [GSYM lemma]
+   \\ SIMP_TAC std_ss [GSYM x64_mem64_APPEND, STAR_ASSOC]
+   \\ SIMP_TAC std_ss [lemma]
+   \\ METIS_TAC [SPEC_FRAME]);
+
+val x64_mem32_WRITE_EXTEND = Q.store_thm("x64_mem32_WRITE_EXTEND",
+   `SPEC m (p * x64_mem32 a (w2w w)) c (q * x64_mem32 a v) ==>
+    SPEC m (p * x64_mem64 a w) c
+           (q * x64_mem64 a ((((63 >< 32) w):word32) @@ v))`,
+   REPEAT STRIP_TAC
+   \\ ONCE_REWRITE_TAC [GSYM lemma]
+   \\ SIMP_TAC std_ss [GSYM x64_mem64_APPEND, STAR_ASSOC]
+   \\ SIMP_TAC std_ss [lemma, lemma2]
+   \\ METIS_TAC [SPEC_FRAME]);
 
 (* ------------------------------------------------------------------------ *)
 
