examples/l3-machine-code/common/stateScript.sml
@@ -301,9 +301,10 @@ val SEP_EQ_STAR = Q.store_thm("SEP_EQ_STAR",
   )
 
 val MAPPED_COMPONENT_INSERT = Q.store_thm("MAPPED_COMPONENT_INSERT",
-   `!P single_c x y map_c.
-     (!a b. (x a = x b) = (a = b)) /\
-     (!c d. single_c c d = {{(x c, y d)}}) /\
+   `!P n x y single_c map_c.
+     (!c d. single_c c d = {set (GENLIST (\i. (x c i, y d i)) n)}) ==>
+     (!a b i j. P a /\ P b /\ i < n /\ j < n ==>
+                ((x a i = x b j) = (a = b) /\ (i = j))) /\
      (!df f. map_c df f =
              {BIGUNION {BIGUNION (single_c c (f c)) | c | c IN df /\ P c}}) ==>
      !f df c d.
@@ -314,7 +315,45 @@ val MAPPED_COMPONENT_INSERT = Q.store_thm("MAPPED_COMPONENT_INSERT",
    \\ match_mp_tac SEP_EQ_STAR
    \\ rewrite_tac [SEP_EQ_SINGLETON, pred_setTheory.BIGUNION_SING,
                    pred_setTheory.DISJOINT_DEF, pred_setTheory.EXTENSION]
-   \\ simp [boolTheory.PULL_EXISTS, combinTheory.APPLY_UPDATE_THM]
+   \\ rw [boolTheory.PULL_EXISTS, combinTheory.APPLY_UPDATE_THM,
+          listTheory.MEM_GENLIST]
+   >- metis_tac []
+   \\ Cases_on `x'`     \\ simp [] (* shouldn't rely on name here *)
+   \\ Cases_on `i < n`  \\ simp []
+   \\ Cases_on `i' < n` \\ simp []
+   \\ metis_tac []
+   )
+
+val cnv = SIMP_CONV (srw_ss()) [DECIDE ``i < 1n = (i = 0)``]
+
+val MAPPED_COMPONENT_INSERT1 = Theory.save_thm("MAPPED_COMPONENT_INSERT1",
+   MAPPED_COMPONENT_INSERT
+   |> Q.SPECL [`K T`, `1n`, `\c i. x c`, `\d i. y d`]
+   |> Conv.CONV_RULE
+        (Conv.STRIP_QUANT_CONV
+           (Conv.RATOR_CONV cnv
+            THENC Conv.RAND_CONV (Conv.RATOR_CONV cnv)
+            THENC REWRITE_CONV [combinTheory.K_THM]))
+   |> Drule.GEN_ALL)
+
+val MAPPED_COMPONENT_INSERT_OPT = Q.store_thm("MAPPED_COMPONENT_INSERT_OPT",
+   `!y x single_c map_c.
+      (!c d. single_c c d = {{(x c,y d)}}) ==>
+      (!a b. (x a = x b) <=> (a = b)) /\
+      (!df f.
+         map_c df f =
+         {BIGUNION {BIGUNION (single_c c (SOME (f c))) | c IN df}}) ==>
+      !f df c d.
+        c IN df ==>
+        (single_c c (SOME d) * map_c (df DELETE c) f = map_c df ((c =+ d) f))`,
+   REPEAT strip_tac
+   \\ asm_rewrite_tac [GSYM SEP_EQ_SINGLETON]
+   \\ match_mp_tac SEP_EQ_STAR
+   \\ rewrite_tac [SEP_EQ_SINGLETON, pred_setTheory.BIGUNION_SING,
+                   pred_setTheory.DISJOINT_DEF, pred_setTheory.EXTENSION]
+   \\ rw [boolTheory.PULL_EXISTS, combinTheory.APPLY_UPDATE_THM]
+   >- metis_tac []
+   \\ Cases_on `x'` \\ simp [] (* shouldn't rely on name here *)
    \\ metis_tac []
    )
 
